Stuff as of 24-04

AVL Tree.v
@@ -1,23 +1,57 @@
 Require Export SfLib.
 Require Import Coq.Numbers.Natural.Peano.NPeano.
 
+Definition blt_nat n1 n2 :=
+	negb (ble_nat n2 n1).
+
+Definition bgt_nat n1 n2 :=
+	negb (ble_nat n1 n2).
+
+Fixpoint contains elem l :=
+	match l with
+	| [] => false
+	| x::xs =>
+		match beq_nat elem x with
+		| true => true
+		| false => contains elem xs
+		end
+	end.
+
+Fixpoint first l :=
+	match l with
+	| nil => 0
+	| x::xs => x
+	end.
+
+Fixpoint last l :=
+	match l with
+	| nil => 0
+	| [x] => x
+	| _::xs => last xs
+	end.
+
 Inductive tree: Type :=
 	| leaf : tree
 	| node : nat -> tree -> tree -> tree.
 	        (* Value -> Left -> Right *)
 
-Definition left (t: tree) := 
-	match t with
-	| leaf => None
-	| node _ leftChild _ => Some leftChild
-	end.
+Inductive sorted : list nat -> Prop :=
+	| empty : sorted []
+	| single : forall n, sorted [n]
+	| more : forall n m xs, n <= m -> sorted (m::xs) -> sorted (n::m::xs).
 
-Definition right (t: tree) := 
-	match t with
-	| leaf => None
-	| node _ _ rightChild => Some rightChild
-	end.
-
+Inductive bst : tree -> Prop :=
+	| bst_leaf : bst leaf
+	| bst_node : forall val rVal lVal llT lrT rlT rrT, 
+		ble_nat lVal val = true -> bgt_nat rVal val = true -> bst (node lVal llT lrT) -> 
+		bst (node rVal lrT rrT) -> bst (node val (node lVal llT lrT) (node rVal rlT rrT))
+	| bst_node_leaf : forall val lVal llT lrT, 
+		ble_nat lVal val = true -> bst (node lVal llT lrT) -> 
+		bst (node val (node lVal llT lrT) leaf)
+	| bst_leaf_node : forall val rVal rlT rrT, 
+		bgt_nat rVal val = true -> bst (node rVal rlT rrT) -> 
+		bst (node val leaf (node rVal rlT rrT))
+	| bst_leaf_leaf : forall val, bst (node val leaf leaf).
 
 Fixpoint height (t: tree) :=
 	match t with
@@ -39,7 +73,6 @@ Example addexample:
 	add 2 (add 5 leaf) = node 5 (node 2 leaf leaf) leaf.
 Proof. reflexivity. Qed.
 
-(*TODO: Look at weights *)
 Fixpoint balance (t : tree) :=
 	match t with
 	| leaf => leaf
@@ -79,14 +112,6 @@ Fixpoint balance (t : tree) :=
 
 Definition insert val t :=
 	balance (add val t).
-
-Example leftexample :
-	left (node 3 leaf (node 2 leaf leaf)) = Some leaf.
-Proof. reflexivity. Qed.
-
-Example rightexample :
-	right (node 3 (node 2 leaf leaf) leaf) = Some leaf.
-Proof. reflexivity. Qed.
 
 Example add_example :
 	add 5 leaf = node 5 leaf leaf.
@@ -134,15 +159,10 @@ Definition Tree :=
 Example inorder_test :
 	inorder Tree = 1::2::5::[].
 Proof. reflexivity. Qed.
-
-Inductive sorted : list nat -> Prop :=
-	| empty : sorted []
-	| single : forall n, sorted [n]
-	| more : forall n m xs, ble_nat n m = true -> sorted (m::xs) -> sorted (n::m::xs).
 	
 Example propsorted :
 	sorted (inorder Tree).
-Proof. simpl. repeat apply more; try reflexivity. apply single. Qed.
+Proof. simpl. repeat apply more; try omega. apply single. Qed.
 
 Example propnonsorted :
 	sorted (1::1::0::[]).
@@ -155,7 +175,15 @@ Proof. reflexivity. Qed.
 Lemma empty_app : forall (l1: list nat) (l2 : list nat),
 	 [] = l1 ++ l2 -> l1 = [] /\ l2 = [].
 Proof.
-	intros. admit.
+	intros. split. 
+		destruct l1. 
+			reflexivity. 
+			inversion H. 
+		destruct l2. 
+			reflexivity. 
+			destruct l1. 
+				inversion H. 
+				inversion H.
 Qed.
 
 Lemma cons_sorted : forall n l,
@@ -166,56 +194,50 @@ Proof.
 		subst. apply H3.
 Qed.
 
-Lemma concat_app_sorted : forall n l1 l2,
-	sorted (n :: l1 ++ l2) -> sorted (n::l1).
+Lemma cons_app_sorted : forall n l1 l2,
+	sorted (n :: l1 ++ l2) -> sorted (n :: l1).
 Proof.
 	intros. inversion H. 
 		subst. apply empty_app in H2. inversion H2. rewrite H0. apply single. 
-		subst. destruct l1.
+		subst. induction l1.
 			apply single.
-			inversion H. subst.
-			apply more. apply H5. simpl in *.  
+			simpl in *. apply more. admit. 
+			replace (l1++[]) with (l1) in H. apply H. rewrite app_nil_r. reflexivity. 
+			apply IHl2. 
 Qed.
 
-Lemma concat_app_sorted' : forall n l1 l2,
+Lemma cons_app_sorted' : forall n l1 l2,
 	sorted (l1 ++ n::l2) -> sorted (n::l2).
 Proof.
 	intros. admit.
 Qed.
 
+Lemma app_sorted : forall l1 l2,
+	last l1 <= first l2 -> sorted l1 -> sorted l2 -> sorted(l1++l2).
+Proof. 
+	intros. induction H0. simpl in *. assumption.
+	destruct l2. simpl in *. apply single. apply more. assumption. assumption.
+	simpl. apply more. assumption. apply IHsorted. assumption.
+Qed.
+
+Lemma sorted_property : forall l1 l2,
+	sorted (l1++l2) -> last l1 <= first l2.
+Proof.
+	intros. destruct l1. simpl. omega. admit.
+Qed.
+
 Lemma sorted_app: forall l1 l2,
-	sorted(l1++l2) -> sorted l1 /\ sorted l2.
+	sorted(l1++l2) -> sorted l1 /\ sorted l2 /\ last l1 <= first l2.
 Proof. 
 	intros. split.  
 		destruct l1. 
 			apply empty.
 			simpl in H. apply concat_app_sorted in H. apply H.
-		destruct l2.
-			apply empty.
-			apply concat_app_sorted' in H. apply H. 
-Qed.
-
-Fixpoint contains elem l :=
-	match l with
-	| [] => false
-	| x::xs =>
-		match beq_nat elem x with
-		| true => true
-		| false => contains elem xs
-		end
-	end.
-
-Lemma app_sorted : forall l1 l2 e1 e2 xs1 xs2,
-	l1 = xs1 ++ [e1] -> l2 = e2::xs2 -> sorted l1 -> sorted l2 -> ble_nat e1 e2 = true -> sorted(l1++l2).
-Proof. Admitted.
-
-Lemma add_insures_contains : forall elem t,
-	 contains elem (inorder (add elem t)) = true.
-Proof. 
-	intros. induction t. 
-		simpl. rewrite <- beq_nat_refl. reflexivity. 
-		simpl. remember (ble_nat elem n) as guard. destruct guard.
-			simpl. admit. admit.
+		split.
+			destruct l2.
+				apply empty.
+				apply concat_app_sorted' in H. apply H. 
+			apply sorted_property in H. apply H.
 Qed.
 
 Theorem cons_app : forall e (l: list nat),
@@ -224,49 +246,11 @@ Proof.
 	intros. simpl. reflexivity.
 Qed.
 
-Definition blt_nat n1 n2 :=
-	negb (ble_nat n2 n1).
-
-Definition bgt_nat n1 n2 :=
-	negb (ble_nat n1 n2).
-
 Lemma inorder_add : forall n t t' x' xs',
 	inorder t' = x'::xs' -> t' = add n t -> inorder (add n t) = x'::xs'.
 Proof.
 	intros. subst. apply H.
 Qed.
-
-Fixpoint valid_bst t :=
-	match t with
-	| leaf => true
-	| node val lChild rChild => 
-		match lChild with
-		| leaf => match rChild with
-			| leaf => true
-			| node rVal rlChild rrChild => andb (andb (bgt_nat rVal val) (valid_bst rlChild)) (valid_bst rrChild)
-			end
-		| node lVal llChild lrChild => match rChild with
-			| leaf => andb (andb (ble_nat lVal val) (valid_bst llChild)) (valid_bst lrChild)
-			| node rVal rlChild rrChild => 
-				andb (andb (andb (ble_nat lVal val) (bgt_nat rVal val))  
-				(andb (valid_bst llChild) (valid_bst lrChild)))
-				(andb (valid_bst rlChild) (valid_bst rrChild))
-			end
-		end
-	end.
-
-Inductive bst : tree -> Prop :=
-	| bst_leaf : bst leaf
-	| bst_node : forall val rVal lVal llT lrT rlT rrT, 
-		ble_nat lVal val = true -> bgt_nat rVal val = true -> bst (node lVal llT lrT) -> 
-		bst (node rVal lrT rrT) -> bst (node val (node lVal llT lrT) (node rVal rlT rrT))
-	| bst_node_leaf : forall val lVal llT lrT, 
-		ble_nat lVal val = true -> bst (node lVal llT lrT) -> 
-		bst (node val (node lVal llT lrT) leaf)
-	| bst_leaf_node : forall val rVal rlT rrT, 
-		bgt_nat rVal val = true -> bst (node rVal rlT rrT) -> 
-		bst (node val leaf (node rVal rlT rrT))
-	| bst_leaf_leaf : forall val, bst (node val leaf leaf).
 
 Definition BigTree :=
 	 node 6 (Tree) (node 10 leaf leaf).
@@ -282,53 +266,53 @@ Example not_bst_prop_example:
 	bst not_bst.
 Proof. unfold not_bst. apply bst_node_leaf. Admitted. (*UNPOSSIBLE*)
 
-Example big_tree_example :
-	valid_bst BigTree = true.
-Proof. reflexivity. Qed.
-
-Example not_bst_example :
-	valid_bst not_bst = false.
-Proof. reflexivity. Qed.
-
-Definition BigTree2 :=
-	node 5 leaf BigTree.
-	
-Example big_tree_2_example:
-	valid_bst BigTree2 = true.
-Proof. reflexivity. Qed.
-
-Lemma add_preserves_bst : forall n t,
-	bst t -> bst (add n t).
+Lemma last_first_sorted : forall n m t,
+	true = ble_nat n m -> last (inorder t) <= m -> last (inorder (add n t)) <= m.
 Proof.
-	intros. induction t.
-		constructor.
-		simpl. remember (ble_nat n n0) as b. destruct b.
-			admit. admit.
+	intros. admit.
 Qed.
 
+Lemma first_last_sorted: forall n m t,
+	false = ble_nat n m -> sorted (inorder (add n t)) -> sorted(m::inorder(add n t)).
+Proof.
+	intros. admit.
+Qed.
 
-(*
-Theorem add_preserves_bst: forall n t,
+Theorem add_preserves_bst': forall n t,
 	sorted (inorder t) -> sorted (inorder (add n t)).
 Proof.
 	intros. induction t. 
 		Case "leaf". apply single.
-		Case "node". simpl in H. apply sorted_app in H. inversion H. simpl. 
+		Case "node". simpl in H. apply sorted_app in H. inversion H. inversion H1. simpl. 
 			remember (ble_nat n n0) as add. destruct add. 
-				simpl. rewrite inorder_add with (t':=add n t1)(x':=batman)(xs':=alfred). remember (add n t1) as addnt1. destruct addnt1. 
-					inversion Heqaddnt1. rewrite inorder_add with (n:=n)(t:=t1)(t':=add n t1). apply app_sorted.
-					apply add_insures_contains. reflexivity. apply IHt1. apply H0. apply H1. symmetry. apply Heqadd. 
-				simpl. apply app_sorted2 with (e1:=n0)(e2:=n)(xs2:=inorder (add n t2)). 
-					simpl. remember (beq_nat n n0) as beqnat. destruct beqnat. 
-						reflexivity. 
-						apply add_insures_contains. reflexivity. apply H0. rewrite <- cons_app. apply spec_split_inorder_add_sort.
-							apply single. apply IHt2. rewrite <- cons_app in H1. apply sorted_app in H1. inversion H1. apply H3.
-							unfold blt_nat. rewrite <- Heqadd. reflexivity. 
+				simpl. apply app_sorted; simpl; try apply last_first_sorted; try assumption. apply IHt1. assumption. 
+				simpl. apply app_sorted. simpl in *. apply H3. assumption. apply first_last_sorted; try assumption. apply IHt2. 
+				apply cons_sorted in H2. apply H2.
 Qed.
-*)
+
+Lemma less_than_or_equal : forall n m,
+	true = ble_nat n m -> n <= m.
+Proof.
+	intros. destruct n. 
+		omega.
+		destruct m. 
+			inversion H.
+			admit.
+Qed.
+
+Theorem insert_preserves_bst : forall n t,
+	sorted (inorder t) -> sorted (inorder (insert n t)).
+Proof.
+	intros. induction t. 
+		simpl. apply single.
+		simpl in H. apply sorted_app in H. inversion H. inversion H1. unfold insert. simpl in *. remember (ble_nat n n0) as add. 
+		destruct add. 
+			
+				
+Qed.
 
 Theorem insert_preserves_balance: forall n t t',
-	t = insert n t' -> ble_nat (height t) (log2 (length (inorder t') + 1)+1) = true.
+	t = insert n t' ->height t <= log2 (length (inorder t') + 1) + 1 = true.
 Proof. 
 	intros. induction t'.
 		Case "leaf". rewrite H. reflexivity.
